fixed syntax errors

Isabelle/Graph.thy
@@ -41,20 +41,22 @@ lemma reachable_trans:
   shows "reachable x z"
   using assms by induct auto
 
-function unite :: "'v \<Rightarrow> 'v \<Rightarrow> 'v env" where
+function unite :: "'v \<Rightarrow> 'v \<Rightarrow> 'v env \<Rightarrow> 'v env" where
   "unite v w e =
       (if (S e v = S e w) then e
       else let r = hd(stack e);
                r'= hd(tl(stack e));
-               e'= e \<lparr> stack := tl(stack e), S := S e (r \<leftarrow> S e r \<union> S e r', r' \<leftarrow> S e r \<union> S e r')\<rparr>
+               joined = S e r \<union> S e r';
+               e'= e \<lparr> stack := tl(stack e), S := (S e) (r := joined, r' := joined)\<rparr>
           in unite v w e')"
+  by pat_completeness auto
 
 function dfs :: "'v \<Rightarrow> 'v env \<Rightarrow> 'v env" and dfss :: "'v \<Rightarrow> 'v set \<Rightarrow> 'v env \<Rightarrow> 'v env" where
   "dfs v e =
-  (let e1 = e1\<lparr>visited := visited e \<union> {v}, stack := (v # stack e)\<rparr>;
-       e' = dfss (succ v) e1
+  (let e1 = e\<lparr>visited := visited e \<union> {v}, stack := (v # stack e)\<rparr>;
+       e' = dfss v (successors v) e1
   in if v = hd(stack e')
-      then e'\<lparr>sccs:=sccs e' \<union> (S e v), explored:=explored e' \<union> (S e u), stack:=tl(stack e')\<rparr>
+      then e'\<lparr>sccs:=sccs e' \<union> {S e v}, explored:=explored e' \<union> (S e v), stack:=tl(stack e')\<rparr>
     else e')"
 | "dfss v vs e =
    (if vs = {} then e
@@ -64,6 +66,27 @@ function dfs :: "'v \<Rightarrow> 'v env \<Rightarrow> 'v env" and dfss :: "'v \
       else if w \<notin> visited e
         then dfs w e
       else unite v w e)))"
+  by pat_completeness (force+)
+
+text \<open>
+  Well-formed environments.
+\<close>
+definition wf_env where "wf_env e \<equiv> True"
+
+text \<open>
+  Precondition for function dfs.
+\<close>
+definition pre_dfs where "pre_dfs v e \<equiv> wf_env e"
+
+text \<open>
+  Precondition for function dfss.
+\<close>
+definition pre_dfss where "pre_dfss v vs e \<equiv> wf_env e"
+
+lemma pre_dfs_pre_dfss:
+  assumes "pre_dfs v e"
+  shows "pre_dfss v (successors v) (e \<lparr> visited := visited e \<union> {v}, stack := v # stack e\<rparr>)"
+  sorry
 
 end
 end
